theories/examples/delim_lang/lang.v
@@ -1,8 +1,10 @@
 From gitrees Require Export prelude.
-
+From stdpp Require Import gmap.
+(* From iris.heap_lang Require Import locations. *)
 Require Import Binding.Resolver Binding.Lib Binding.Set Binding.Auto Binding.Env.
-(* Require Import FunctionalExtensionality. *)
 
+(* Definition loc : Set := locations.loc. *)
+(* Global Instance loc_dec_eq (l l' : loc) : Decision (l = l') := _. *)
 Variant nat_op := Add | Sub | Mult.
 
 Inductive expr {X : Set} :=
@@ -19,10 +21,15 @@ Inductive expr {X : Set} :=
 (* The effects *)
 | Shift (e : @expr (inc X)) : expr
 | Reset (e : expr) : expr
+(* | Alloc (e : expr) : expr *)
+(* | Deref (e : expr) : expr *)
+(* | Assign (e₁ : expr) (e₂ : expr) : expr *)
 with val {X : Set} :=
 | LitV (n : nat) : val
 | RecV (e : @expr (inc (inc X))) : val
 | ContV (k : cont) : val
+(* | LocV (l : loc) : val *)
+(* | UnitV : val *)
 with cont {X : Set} :=
 | END : cont
 | IfK (e1 : expr) (e2 : expr) : cont -> cont
@@ -31,11 +38,14 @@ with cont {X : Set} :=
 | AppContLK (v : val) : cont -> cont (* ◻ v *)
 | AppContRK (e : expr) : cont -> cont (* e ◻ *)
 | NatOpLK (op : nat_op) (v : val) : cont -> cont (* ◻ + v *)
-| NatOpRK (op : nat_op) (e : expr) : cont -> cont. (* e + ◻ *)
-
+| NatOpRK (op : nat_op) (e : expr) : cont -> cont (* e + ◻ *)
+(* | AllocK : cont → cont *)
+(* | DerefK : cont → cont *)
+(* | AssignRK (e : expr) : cont → cont (* E <- e *) *)
+(* | AssignLK (v : val) : cont → cont (* v <- E *) *)
+.
 (* conts are inside-out contexts: eg
  IfK e1 e2 (AppLK v ◻) ==> App (if ◻ then e1 else e2) v*)
-
 
 Arguments val X%bind : clear implicits.
 Arguments expr X%bind : clear implicits.
@@ -53,6 +63,9 @@ Fixpoint emap {A B : Set} (f : A [→] B) (e : expr A) : expr B :=
   | If e₁ e₂ e₃ => If (emap f e₁) (emap f e₂) (emap f e₃)
   | Shift e => Shift (emap (f ↑) e)
   | Reset e => Reset (emap f e)
+  (* | Alloc e => Alloc (emap f e) *)
+  (* | Deref e => Deref (emap f e) *)
+  (* | Assign e₁ e₂ => Assign (emap f e₁) (emap f e₂) *)
   end
 with
 vmap {A B : Set} (f : A [→] B) (v : val A) : val B :=
@@ -60,6 +73,8 @@ vmap {A B : Set} (f : A [→] B) (v : val A) : val B :=
   | LitV n => LitV n
   | RecV e => RecV (emap ((f ↑) ↑) e)
   | ContV k => ContV (kmap f k)
+  (* | LocV l => LocV l *)
+  (* | UnitV => UnitV *)
   end
 with kmap {A B : Set} (f : A [→] B) (K : cont A) : cont B :=
    match K with
@@ -71,6 +86,10 @@ with kmap {A B : Set} (f : A [→] B) (K : cont A) : cont B :=
    | AppContRK e k => AppContRK (emap f e) (kmap f k)
    | NatOpLK op v k => NatOpLK op (vmap f v) (kmap f k)
    | NatOpRK op e k => NatOpRK op (emap f e) (kmap f k)
+   (* | AllocK k => AllocK (kmap f k) *)
+   (* | DerefK k => DerefK (kmap f k) *)
+   (* | AssignRK e k => AssignRK (emap f e) (kmap f k) *)
+   (* | AssignLK v k => AssignLK (vmap f v) (kmap f k) *)
    end.
 
 
@@ -90,6 +109,9 @@ Fixpoint ebind {A B : Set} (f : A [⇒] B) (e : expr A) : expr B :=
   | If e₁ e₂ e₃ => If (ebind f e₁) (ebind f e₂) (ebind f e₃)
   | Shift e => Shift (ebind (f ↑) e)
   | Reset e => Reset (ebind f e)
+  (* | Alloc e => Alloc (ebind f e) *)
+  (* | Deref e => Deref (ebind f e) *)
+  (* | Assign e₁ e₂ => Assign (ebind f e₁) (ebind f e₂) *)
   end
 with
 vbind {A B : Set} (f : A [⇒] B) (v : val A) : val B :=
@@ -97,6 +119,8 @@ vbind {A B : Set} (f : A [⇒] B) (v : val A) : val B :=
   | LitV n => LitV n
   | RecV e => RecV (ebind ((f ↑) ↑) e)
   | ContV k => ContV (kbind f k)
+  (* | LocV l => LocV l *)
+  (* | UnitV => UnitV *)
   end
 with kbind {A B : Set} (f : A [⇒] B) (K : cont A) : cont B :=
    match K with
@@ -108,6 +132,10 @@ with kbind {A B : Set} (f : A [⇒] B) (K : cont A) : cont B :=
    | AppContRK e k => AppContRK (ebind f e) (kbind f k)
    | NatOpLK op v k => NatOpLK op (vbind f v) (kbind f k)
    | NatOpRK op e k => NatOpRK op (ebind f e) (kbind f k)
+   (* | AllocK k => AllocK (kbind f k) *)
+   (* | DerefK k => DerefK (kbind f k) *)
+   (* | AssignRK e k => AssignRK (ebind f e) (kbind f k) *)
+   (* | AssignLK v k => AssignLK (vbind f v) (kbind f k) *)
    end.
 
 #[export] Instance BindCore_expr : BindCore expr := @ebind.
@@ -287,8 +315,11 @@ Fixpoint fill {X : Set} (K : cont X) (e : expr X) : expr X :=
   | AppContRK el K => fill K (AppCont el e)
   | NatOpLK op v K => fill K (NatOp op e (Val v))
   | NatOpRK op el K => fill K (NatOp op el e)
+  (* | AllocK K => fill K (Alloc e) *)
+  (* | DerefK K => fill K (Deref e) *)
+  (* | AssignRK e' K => fill K (Assign e e') *)
+  (* | AssignLK v K => fill K (Assign (Val v) e) *)
   end.
-
 
 (*** Continuation operations *)
 
@@ -314,6 +345,10 @@ Fixpoint cont_compose {S} (K1 K2 : cont S) : cont S :=
   | AppContRK e K => AppContRK e (cont_compose K1 K)
   | NatOpLK op v K => NatOpLK op v (cont_compose K1 K)
   | NatOpRK op e K => NatOpRK op e (cont_compose K1 K)
+  (* | AllocK K => AllocK (cont_compose K1 K) *)
+  (* | DerefK K => DerefK (cont_compose K1 K) *)
+  (* | AssignRK e' K => AssignRK e' (cont_compose K1 K) *)
+  (* | AssignLK v K => AssignLK v (cont_compose K1 K) *)
   end.
 
 Lemma fill_comp {S} (K1 K2 : cont S) e : fill (cont_compose K1 K2) e = fill K1 (fill K2 e).
@@ -322,20 +357,19 @@ Proof.
   intros H K1 e; simpl; by rewrite H.
 Qed.
 
-
 Lemma fill_not_val : ∀ {S} K (e : expr S), to_val e = None → to_val (fill K e) = None.
 Proof.
   intros S K e. rewrite !eq_None_not_Some.
   eauto using fill_val.
 Qed.
 
-
 (*** Abstract Machine semantics *)
 
 Definition Mcont {S} := list $ cont S.
+(* Definition state X := gmap loc (val X). *)
 
 Variant config {S} : Type :=
-  | Ceval : expr S -> cont S -> @Mcont S -> config
+  | Ceval : expr S -> cont S -> @Mcont S → config
   | Ccont : cont S -> val S -> @Mcont S -> config
   | Cmcont : @Mcont S -> val S -> config
   | Cexpr : expr S -> config
@@ -344,183 +378,127 @@ Variant config {S} : Type :=
 Reserved Notation "c '===>' c' / nm"
   (at level 40, c', nm at level 30).
 
-Variant Cred {S : Set} : config -> config -> (nat * nat) -> Prop :=
+Variant Cred {S : Set} : config (* * state S *) -> config (* * state S *) -> (nat * nat) -> Prop :=
 
   (* init *)
-  | Ceval_init : forall (e : expr S),
-      Cexpr e ===> Ceval e END [] / (0,0)
+  | Ceval_init : forall (e : expr S) (* σ *),
+  (Cexpr e(* , σ *)) ===> (Ceval e END [](* , σ *)) / (0,0)
 
-  (* eval *)
-  | Ceval_val : forall v k mk,
-      Ceval (Val v) k mk ===> Ccont k v mk / (0,0)
+(* eval *)
+| Ceval_val : forall v k mk (* σ *),
+  (Ceval (Val v) k mk(* , σ *)) ===> (Ccont k v mk(* , σ *)) / (0,0)
 
-  | Ceval_app : forall e0 e1 k mk,
-      Ceval (App e0 e1) k mk ===> Ceval e1 (AppRK e0 k) mk / (0,0)
+| Ceval_app : forall e0 e1 k mk (* σ *),
+  (Ceval (App e0 e1) k mk(* , σ *)) ===> (Ceval e1 (AppRK e0 k) mk(* , σ *)) / (0,0)
 
-  | Ceval_app_cont : forall e0 e1 k mk,
-      Ceval (AppCont e0 e1) k mk ===> Ceval e1 (AppContRK e0 k) mk / (0,0)
+| Ceval_app_cont : forall e0 e1 k mk (* σ *),
+  (Ceval (AppCont e0 e1) k mk(* , σ *)) ===> (Ceval e1 (AppContRK e0 k) mk(* , σ *)) / (0,0)
 
-  | Ceval_natop : forall op e0 e1 k mk,
-      Ceval (NatOp op e0 e1) k mk ===> Ceval e1 (NatOpRK op e0 k) mk / (0,0)
+| Ceval_natop : forall op e0 e1 k mk (* σ *),
+  (Ceval (NatOp op e0 e1) k mk(* , σ *)) ===> (Ceval e1 (NatOpRK op e0 k) mk(* , σ *)) / (0,0)
 
-  | Ceval_if : forall eb et ef k mk,
-      Ceval (If eb et ef) k mk ===> Ceval eb (IfK et ef k) mk / (0,0)
+| Ceval_if : forall eb et ef k mk (* σ *),
+  (Ceval (If eb et ef) k mk(* , σ *)) ===> (Ceval eb (IfK et ef k) mk(* , σ *)) / (0,0)
 
-  | Ceval_reset : forall e k mk,
-      Ceval (Reset e) k mk ===> Ceval e END (k :: mk) / (1, 1)
+| Ceval_reset : forall e k mk (* σ *),
+  (Ceval (Reset e) k mk(* , σ *)) ===> (Ceval e END (k :: mk)(* , σ *)) / (1, 1)
 
-  | Ceval_shift : forall (e : expr $ inc S) k mk,
-      Ceval (Shift e) k mk ===>
-        Ceval (subst (Inc := inc) e (Val $ ContV k))
-        END mk / (1, 1)
+| Ceval_shift : forall (e : expr $ inc S) k mk (* σ *),
+  (Ceval (Shift e) k mk(* , σ *)) ===>
+    (Ceval (subst (Inc := inc) e (Val $ ContV k)) END mk(* , σ *)) / (1, 1)
 
-  (* cont *)
-  | Ccont_end : forall v mk,
-      Ccont END v mk ===> Cmcont mk v / (0,0)
+(* cont *)
+| Ccont_end : forall v mk (* σ *),
+  (Ccont END v mk(* , σ *)) ===> (Cmcont mk v(* , σ *)) / (0,0)
 
-  | Ccont_appr : forall e v k mk,
-      Ccont (AppRK e k) v mk ===> Ceval e (AppLK v k) mk / (0, 0)
+| Ccont_appr : forall e v k mk (* σ *),
+  (Ccont (AppRK e k) v mk(* , σ *)) ===> (Ceval e (AppLK v k) mk(* , σ *)) / (0, 0)
 
-  | Ccont_app_contr : forall e v k mk,
-      Ccont (AppContRK e k) v mk ===> Ceval e (AppContLK v k) mk / (0, 0)
+| Ccont_app_contr : forall e v k mk (* σ *),
+  (Ccont (AppContRK e k) v mk(* , σ *)) ===> (Ceval e (AppContLK v k) mk(* , σ *)) / (0, 0)
 
-  | Ccont_appl : forall e v k mk,
-      Ccont (AppLK v k) (RecV e) mk ===>
-        Ceval (subst (Inc := inc)
-                 (subst (F := expr) (Inc := inc) e
-                    (Val (shift (Inc := inc) v)))
-                 (Val (RecV e))) k mk / (1, 0)
+| Ccont_appl : forall e v k mk (* σ *),
+  (Ccont (AppLK v k) (RecV e) mk(* , σ *)) ===>
+    (Ceval (subst (Inc := inc)
+              (subst (F := expr) (Inc := inc) e
+                 (Val (shift (Inc := inc) v)))
+              (Val (RecV e))) k mk(* , σ *)) / (1, 0)
 
-  | Ccont_cont : forall v k k' mk,
-      Ccont (AppContLK v k) (ContV k') mk ===>
-        Ccont k' v (k :: mk) / (2, 1)
+| Ccont_cont : forall v k k' mk (* σ *),
+  (Ccont (AppContLK v k) (ContV k') mk(* , σ *)) ===>
+    (Ccont k' v (k :: mk)(* , σ *)) / (2, 1)
 
-  | Ccont_if : forall et ef n k mk,
-      Ccont (IfK et ef k) (LitV n) mk ===>
-        Ceval (if (n =? 0) then ef else et) k mk / (0, 0)
+| Ccont_if : forall et ef n k mk (* σ *),
+  (Ccont (IfK et ef k) (LitV n) mk(* , σ *)) ===>
+    (Ceval (if (n =? 0) then ef else et) k mk(* , σ *)) / (0, 0)
 
-  | Ccont_natopr : forall op e v k mk,
-      Ccont (NatOpRK op e k) v mk ===>
-        Ceval e (NatOpLK op v k) mk / (0, 0)
+| Ccont_natopr : forall op e v k mk (* σ *),
+  (Ccont (NatOpRK op e k) v mk(* , σ *)) ===>
+    (Ceval e (NatOpLK op v k) mk(* , σ *)) / (0, 0)
 
-  | Ccont_natopl : forall op v0 v1 v2 k mk,
-      nat_op_interp op v0 v1 = Some v2 ->
-      Ccont (NatOpLK op v1 k) v0 mk ===>
-        Ceval (Val v2) k mk / (0,0)
+| Ccont_natopl : forall op v0 v1 v2 k mk (* σ *),
+  nat_op_interp op v0 v1 = Some v2 ->
+  (Ccont (NatOpLK op v1 k) v0 mk(* , σ *)) ===>
+    (Ceval (Val v2) k mk(* , σ *)) / (0,0)
 
-  (* meta-cont *)
-  | Cmcont_cont : forall k mk v,
-      Cmcont (k :: mk) v ===> Ccont k v mk / (1,1)
+(* meta-cont *)
+| Cmcont_cont : forall k mk v (* σ *),
+  (Cmcont (k :: mk) v(* , σ *)) ===> (Ccont k v mk(* , σ *)) / (1,1)
 
-  | Cmcont_ret : forall v,
-      Cmcont [] v ===> Cret v / (1, 1)
+| Cmcont_ret : forall v (* σ *),
+  (Cmcont [] v(* , σ *)) ===> (Cret v(* , σ *)) / (1, 1)
 
+(* | Ceval_assign : forall e0 e1 k mk σ, *)
+(*   (Ceval (Assign e0 e1) k mk, σ) ===> (Ceval e1 (AssignRK e0 k) mk, σ) / (0, 0) *)
+
+(* | Ccont_assignr : forall e v k mk σ, *)
+(*   (Ccont (AssignRK e k) v mk, σ) ===> (Ceval e (AssignLK v k) mk, σ) / (0, 0) *)
+
+(* | Ccont_assignl : forall l v' k mk σ, *)
+(*   (Ccont (AssignLK (LocV l) k) v' mk, σ) ===> *)
+(*     (Ceval (Val UnitV) k mk, <[l:=v']>σ) / (0, 1) *)
+
+(* | Ceval_alloc : forall e k mk σ, *)
+(*   (Ceval (Alloc e) k mk, σ) ===> (Ceval e (AllocK k) mk, σ) / (0, 0) *)
+
+(* | Ceval_allock : ∀ l v k mk σ, *)
+(*   σ !! l = None -> *)
+(*   (Ccont (AllocK k) v mk, σ) ===> *)
+(*     (Ceval (Val (LocV l)) k mk, <[l:=v]>σ) / (0, 1) *)
+
+(* | Ceval_deref : forall e k mk σ, *)
+(*   (Ceval (Deref e) k mk, σ) ===> (Ceval e (DerefK k) mk, σ) / (0, 0) *)
+
+(* | Ceval_derefk : ∀ l v k mk σ, *)
+(*   σ !! l = Some v -> *)
+(*   (Ccont (DerefK k) (LocV l) mk, σ) ===> *)
+(*     (Ceval (Val v) k mk, σ) / (0, 1) *)
 where "c ===> c' / nm" := (Cred c c' nm).
 
 Arguments Mcont S%bind : clear implicits.
 Arguments config S%bind : clear implicits.
 
-Inductive steps {S} : config S -> config S -> (nat * nat) -> Prop :=
+Inductive steps {S} : config S (* * state S *) -> config S (* * state S *) -> (nat * nat) -> Prop :=
 | steps_zero : forall c,
-    steps c c (0,0)
-| steps_many : forall c1 c2 c3 n m n' m',
-    c1 ===> c2 / (n,m) ->
-    steps c2 c3 (n',m') ->
-    steps c1 c3 (n+n',m+m').
+  steps c c (0, 0)
+| steps_many : forall c1 c2 c3 n m n' m' n'' m'',
+  n'' = n + n' -> m'' = m + m' ->
+  c1 ===> c2 / (n, m) ->
+  steps c2 c3 (n', m') ->
+  steps c1 c3 (n'', m'').
 
 Definition meta_fill {S} (mk : Mcont S) e :=
   fold_left (λ e k, fill k e) mk e.
 
-(*** Type system *)
-(* Type system from [Filinski, Danvy 89] : A Functional Abstraction of Typed Contexts *)
-
 Coercion Val : val >-> expr.
-
-Inductive ty :=
-| Tnat : ty
-| Tarr : ty -> ty -> ty -> ty -> ty
-| TarrCont : ty -> ty -> ty -> ty -> ty.
-
-
-(* Notation "'T' τ '/' α '->' σ '/' β" := (Tarr τ α σ β) (at level 99, only parsing). *)
-(* Notation "τ '/' α '→k' σ '/' β" := (TarrCont τ α σ β) (at level 60). *)
-
-(* Reserved Notation " Γ , α ⊢ e : τ , β" *)
-(*   (at level 90, e at next level, τ at level 20, no associativity). *)
-
-(* Inductive typed {S : Set} (Γ : S -> ty) : ty -> expr S -> ty -> ty -> Prop := *)
-
-(* | typed_Lit α n : *)
-(*   Γ, α ⊢ (LitV n) : Tnat, α *)
-
-(* | typed_Rec (δ σ τ α β : ty) (e : expr (inc (inc S))) : *)
-(*     (Γ ▹ (Tarr  σ α τ β) ▹ σ) , α ⊢ e : τ , β -> *)
-(*     Γ,δ ⊢ (RecV e) : (Tarr σ α τ β) , δ *)
-
-(* | typed_Cont (δ σ τ α : ty) (k : cont S) : *)
-(*   typed_cont Γ α k (TarrCont σ α τ α) α -> *)
-(*   Γ,δ ⊢ (ContV k) : (TarrCont σ α τ α) , δ *)
-
-(* with typed_cont {S : Set} (Γ : S -> ty) : ty -> cont S -> ty -> ty -> Prop := *)
-
-(* | typed_END τ α δ : *)
-(*   typed_cont Γ δ END (TarrCont τ α τ α) δ *)
-
-(* | typed_IfK τ τ' α ε e1 e2 : *)
-(*   Γ, α ⊢ e1 : τ, α -> *)
-(*   Γ, α ⊢ e2 : τ, α -> *)
-(*   typed_cont Γ α K  *)
-(*   typed_cont Γ α (IfK e1 e2 K) (TarrCont Tnat ε τ' ε) α *)
-
-(* where "Γ , α ⊢ e : τ , β" := (typed Γ α e τ β). *)
-
-(* | typed_Val (τ : ty) (v : val S)  : *)
-(*   typed_val Γ v τ → *)
-(*   typed Γ (Val v) τ *)
-(* | typed_Var (τ : ty) (v : S)  : *)
-(*   Γ v = τ → *)
-(*   typed Γ (Var v) τ *)
-(* | typed_App (τ1 τ2 : ty) e1 e2 : *)
-(*   typed Γ e1 (Tarr τ1 τ2) → *)
-(*   typed Γ e2 τ1 → *)
-(*   typed Γ (App e1 e2) τ2 *)
-(* | typed_NatOp e1 e2 op : *)
-(*   typed Γ e1 Tnat → *)
-(*   typed Γ e2 Tnat → *)
-(*   typed Γ (NatOp op e1 e2) Tnat *)
-(* | typed_If e0 e1 e2 τ : *)
-(*   typed Γ e0 Tnat → *)
-(*   typed Γ e1 τ → *)
-(*   typed Γ e2 τ → *)
-(*   typed Γ (If e0 e1 e2) τ *)
-(* | typed_Shift (e : expr (inc S)) τ : *)
-(*   typed (Γ ▹ Tcont τ) e τ -> *)
-(*   typed Γ (Shift e) τ *)
-(* | typed_App_Cont (τ τ' : ty) e1 e2 : *)
-(*   typed Γ e1 (Tcont τ) -> *)
-(*   typed Γ e2 τ -> *)
-(*   typed Γ (App e1 e2) τ' *)
-(* | type_Reset e τ : *)
-(*   typed Γ e τ -> *)
-(*   typed Γ (Reset e) τ *)
-(* (* CHECK *) *)
-(* with typed_val {S : Set} (Γ : S -> ty) : ty -> val S -> ty -> ty -> Prop := *)
-(* | typed_Lit n : *)
-(*   typed_val Γ (LitV n) Tnat *)
-(* | typed_RecV (τ1 τ2 : ty) (e : expr (inc (inc S))) : *)
-(*   typed (Γ ▹ (Tarr τ1 τ2) ▹ σ) e τ2 → *)
-(*   typed_val Γ (RecV e) (Tarr τ1 τ2) *)
-(* . *)
 
 (*** Notations *)
 
 Declare Scope syn_scope.
 Delimit Scope syn_scope with syn.
 
-
+(* Coercion LocV : loc >-> val. *)
 Coercion App : expr >-> Funclass.
-(* Coercion AppLK : expr >-> Funclass. *)
-(* Coercion AppRK : expr >-> Funclass. *)
 
 Class AsSynExpr (F : Set -> Type) := { __asSynExpr : ∀ S, F S -> expr S }.
 
@@ -558,38 +536,10 @@ Global Instance IfNotationK {S : Set} {F G : Set -> Type} `{AsSynExpr F, AsSynEx
   __if K e₂ e₃ := cont_compose K (IfK (__asSynExpr e₂) (__asSynExpr e₃) END)
   }.
 
-
-(* Class OutputNotation (A B : Type) := { __output : A -> B }. *)
-
-(* Global Instance OutputNotationExpr {S : Set} {F : Set -> Type} `{AsSynExpr F} : OutputNotation (F S) (expr S) := { *)
-(*   __output e := Output (__asSynExpr e) *)
-(*   }. *)
-
-(* Global Instance OutputNotationK {S : Set} : OutputNotation (cont S) (cont S) := { *)
-(*   __output K := cont_compose K (OutputK END) *)
-(*   }. *)
-
 Class ResetNotation (A B : Type) := { __reset : A -> B }.
 
 Global Instance ResetNotationExpr {S : Set} {F : Set -> Type} `{AsSynExpr F} :
   ResetNotation (F S) (expr S) := { __reset e := Reset (__asSynExpr e) }.
-
-(* Global Instance ResetNotationK {S : Set} : ResetNotation (cont S) (cont S) := *)
-(*   { __reset K := cont_compose K (ResetK END) }. *)
-
-(* Class ThrowNotation (A B C : Type) := { __throw : A -> B -> C }. *)
-
-(* Global Instance ThrowNotationExpr {S : Set} {F G : Set -> Type} `{AsSynExpr F, AsSynExpr G} : ThrowNotation (F S) (G S) (expr S) := { *)
-(*   __throw e₁ e₂ := Throw (__asSynExpr e₁) (__asSynExpr e₂) *)
-(*   }. *)
-
-(* Global Instance ThrowNotationLK {S : Set} {F : Set -> Type} `{AsSynExpr F} : ThrowNotation (cont S) (F S) (cont S) := { *)
-(*   __throw K e₂ := ThrowLK K (__asSynExpr e₂) *)
-(*   }. *)
-
-(* Global Instance ThrowNotationRK {S : Set} : ThrowNotation (val S) (cont S) (cont S) := { *)
-(*   __throw v K := ThrowRK v K *)
-(*   }. *)
 
 Class AppNotation (A B C : Type) := { __app : A -> B -> C }.
 
@@ -619,6 +569,45 @@ Global Instance AppContNotationRK {S : Set} {F : Set -> Type} `{AsSynExpr F} : A
   __app_cont e K := cont_compose K (AppContRK (__asSynExpr e) END)
   }.
 
+(* Class AllocNotation (A B : Type) := { __alloc : A -> B }. *)
+(* Notation "'alloc' e" := (__alloc e%syn) (at level 61) : syn_scope. *)
+
+(* Global Instance AllocNotationExpr {S : Set} {F : Set -> Type} `{AsSynExpr F} : *)
+(*   AllocNotation (F S) (expr S) := { __alloc e := Alloc (__asSynExpr e) }. *)
+
+(* Global Instance AllocNotationK {S : Set} : AllocNotation (cont S) (cont S) := *)
+(*   { __alloc K := AllocK K }. *)
+
+(* Class DerefNotation (A B : Type) := { __deref : A -> B }. *)
+(* Notation "'!' e" := (__deref e%syn) (at level 61) : syn_scope. *)
+
+(* Global Instance DerefNotationExpr {S : Set} {F : Set -> Type} `{AsSynExpr F} : *)
+(*   DerefNotation (F S) (expr S) := { __deref e := Deref (__asSynExpr e) }. *)
+
+(* Global Instance DerefNotationK {S : Set} : DerefNotation (cont S) (cont S) := *)
+(*   { __deref K := DerefK K }. *)
+
+(* Class AssignNotation (A B C : Type) := { __assign : A -> B -> C }. *)
+(* (* <- !!! *) *)
+(* Notation "x '<-' y" := (__assign x%syn y%syn) *)
+(*                         (at level 40, y at next level, left associativity) *)
+(*     : syn_scope. *)
+
+(* Global Instance AssignNotationExpr {S : Set} {F G : Set -> Type} *)
+(*   `{AsSynExpr F, AsSynExpr G} : AssignNotation (F S) (G S) (expr S) := { *)
+(*   __assign e₁ e₂ := Assign (__asSynExpr e₁) (__asSynExpr e₂) *)
+(*   }. *)
+
+(* Global Instance AssignNotationLK {S : Set} *)
+(*   : AssignNotation (cont S) (val S) (cont S) := { *)
+(*     __assign K v := AssignLK v K *)
+(*   }. *)
+
+(* Global Instance AssignNotationRK {S : Set} {F : Set -> Type} `{AsSynExpr F} *)
+(*   : AssignNotation (F S) (cont S) (cont S) := { *)
+(*     __assign e K := AssignRK (__asSynExpr e) K *)
+(*   }. *)
+
 Notation of_val := Val (only parsing).
 
 Notation "x '⋆' y" := (__app x%syn y%syn) (at level 40, y at next level, left associativity) : syn_scope.
@@ -627,162 +616,58 @@ Notation "x '+' y" := (__op x%syn Add y%syn) : syn_scope.
 Notation "x '-' y" := (__op x%syn Sub y%syn) : syn_scope.
 Notation "x '*' y" := (__op x%syn Mult y%syn) : syn_scope.
 Notation "'if' x 'then' y 'else' z" := (__if x%syn y%syn z%syn) : syn_scope.
-(* Notation "'output' x" := (__output x%syn) (at level 60) : syn_scope. *)
-(* Notation "'throw' e₁ e₂" := (__throw e₁%syn e₂%syn) (at level 60) : syn_scope. *)
 Notation "'#' n" := (LitV n) (at level 60) : syn_scope.
-(* Notation "'input'" := (Input) : syn_scope. *)
 Notation "'rec' e" := (RecV e%syn) (at level 60) : syn_scope.
 Notation "'shift/cc' e" := (Shift e%syn) (at level 60) : syn_scope.
 Notation "'reset' e" := (Reset e%syn) (at level 60) : syn_scope.
-(* Notation "'cont' K" := (ContV K%syn) (at level 60) : syn_scope. *)
 Notation "'$' fn" := (set_pure_resolver fn) (at level 60) : syn_scope.
-(* Notation "□" := (EmptyK) : syn_scope. *)
 Notation "K '⟪' e '⟫'" := (fill K%syn e%syn) (at level 60) : syn_scope.
-
-
-(* Notation "'lam' e" := (LamV e%syn) (at level 60) : syn_scope. *)
-
-(* Definition LetE {S : Set} (e : expr S) (e' : expr (inc S)) : expr S := *)
-(*   App (LamV e') (e). *)
-
-(* Notation "'let_' e₁ 'in' e₂" := (LetE e₁%syn e₂%syn) (at level 60, right associativity) : syn_scope. *)
-
-(* Definition SeqE {S : Set} (e e' : expr S) : expr S := *)
-(*   App (LamV (shift e)) e'. *)
-
-(* Notation "e₁ ';;' e₂" := (SeqE e₁%syn e₂%syn) : syn_scope. *)
-
-Declare Scope typ_scope.
-Delimit Scope typ_scope with typ.
-
-Notation "'ℕ'" := (Tnat) (at level 1) : typ_scope.
-Notation "A →ₜ B" := (Tarr A%typ B%typ)
-                       (right associativity, at level 60) : typ_scope.
-(* Notation "A 'Cont'" := (Tcont A%typ) *)
-(*                          (at level 60) : typ_scope. *)
-
-Declare Scope typing_scope.
-Delimit Scope typing_scope with typing.
-
-Class TypingNotation (A B C : Type) := { __typing : A -> B -> C -> Prop }.
-
-Notation "Γ ⊢ e : τ" := (__typing Γ e%syn τ%typ) (at level 70, e at level 60) : typing_scope.
-
-(* Global Instance TypingNotationExpr {S : Set} {F : Set -> Type} `{AsSynExpr F} : TypingNotation (S -> ty) (F S) ty := { *)
-(*     __typing Γ e τ := typed Γ (__asSynExpr e) τ *)
-(*   }. *)
-
-(* Global Instance TypingNotationVal {S : Set} : TypingNotation (S -> ty) (val S) ty := { *)
-(*     __typing Γ e τ := typed_val Γ e τ *)
-(*   }. *)
 
 Module SynExamples.
 
   Open Scope syn_scope.
 
-  Example test1 : expr (inc ∅) := ($ 0).
-  Example test2 : val ∅ := (rec (if ($ 1) then # 1 else # 0)).
-  (* Example test21 : val ∅ := (lam (if ($ 0) then # 1 else #0)). *)
-  Example test3 : expr ∅ := (shift/cc (rec ($ 0))).
-  Example test4 : expr ∅ := ((# 1) + (# 0)).
-  Example test5 : val ∅ := (rec (if ($ 1) then # 1 else (($ 0) ⋆ (($ 1) - (# 1))))).
-  Example test6 : expr (inc (inc ∅)) := ($ 0) ⋆ ($ 1).
-  (* Example test7 : expr ∅ := (let_ ((rec (if ($ 1) then # 1 else (($ 0) ⋆ (($ 1) - (# 1))))) ⋆ (# 5)) in (output ($ 0))). *)
-
-  Open Scope typing_scope.
-
-  (* Example test8 : Prop := (empty_env ⊢ (# 0) : ℕ). *)
+  Example test1 : expr (inc ∅) := $0.
+  Example test2 : expr (inc (inc ∅)) := ($0) ⋆ $1.
+  Example test3 : expr ∅ := (rec (reset (shift/cc (($0) @k $1)))).
+  Example test4 : expr ∅ :=
+    (rec (if ($0) then #1 else (($0) ⋆ (($0) - #1)))).
+  (* Example test5 : expr ∅ := *)
+  (*   ((alloc #1) <- #2). *)
+  (* Example test6 : expr ∅ := *)
+  (*   (! alloc #1). *)
+  (* Example test7 : *)
+  (*   (∃ (ℓ : loc), *)
+  (*      steps (Cexpr (! alloc #1), empty) (Cret (#1 : val ∅), <[ℓ:=#1]>∅%stdpp) (1, 3)). *)
+  (* Proof. *)
+  (*   set (ℓ := (fresh (dom (∅%stdpp : state ∅)))). *)
+  (*   exists ℓ. *)
+  (*   eapply steps_many with _ 0 0 1 3; first reflexivity; first reflexivity; *)
+  (*     first apply Ceval_init. *)
+  (*   eapply steps_many with _ _ _ 1 3; [| | apply Ceval_deref |]; *)
+  (*     first reflexivity; first reflexivity. *)
+  (*   eapply steps_many with _ _ _ 1 3; [| | apply Ceval_alloc |]; *)
+  (*     first reflexivity; first reflexivity. *)
+  (*   eapply steps_many with _ _ _ 1 3; [| | apply Ceval_val |]; *)
+  (*     first reflexivity; first reflexivity. *)
+  (*   eapply steps_many with _ _ _ 1 2; [| | apply (Ceval_allock ℓ) |]; *)
+  (*     first reflexivity; first reflexivity; first set_solver. *)
+  (*   eapply steps_many with _ _ _ 1 2; [| | apply Ceval_val |]; *)
+  (*     first reflexivity; first reflexivity. *)
+  (*   eapply steps_many with _ _ _ 1 _; [| | eapply (Ceval_derefk ℓ (LitV 1)) |]; *)
+  (*     first reflexivity; first reflexivity; first set_solver. *)
+  (*   eapply steps_many with _ _ _ 1 1; [| | apply Ceval_val |]; *)
+  (*     first reflexivity; first reflexivity. *)
+  (*   eapply steps_many with _ _ _ 1 1; [| | apply Ccont_end |]; *)
+  (*     first reflexivity; first reflexivity. *)
+  (*   eapply steps_many with _ _ _ 0 0; [| | apply Cmcont_ret |]; *)
+  (*     first reflexivity; first reflexivity. *)
+  (*   apply steps_zero. *)
+  (* Qed. *)
+  Example test8 : expr (inc ∅) := ($ 0).
+  Example test9 : val ∅ := (rec (if ($ 1) then # 1 else # 0)).
+  Example test10 : expr ∅ := (shift/cc (rec ($ 0))).
+  Example test11 : expr ∅ := ((# 1) + (# 0)).
+  Example test12 : val ∅ := (rec (if ($ 1) then # 1 else (($ 0) ⋆ (($ 1) - (# 1))))).
+  Example test13 : expr (inc (inc ∅)) := ($ 0) ⋆ ($ 1).
 End SynExamples.
-
-(* Definition compute_head_step {S} *)
-(*   (e : expr S) (K : cont S) : *)
-(*   option (expr S * cont S * (nat * nat)) := *)
-(*   match e with *)
-(*   | (App (Val (RecV e1)) (Val v2)) => *)
-(*       Some ((subst (Inc := inc) ((subst (F := expr) (Inc := inc) e1) *)
-(*                                    (Val (shift (Inc := inc) v2))) *)
-(*                (Val (RecV e1))), K, (1,0)) *)
-(*   (* | Input => *) *)
-(*   (*     let '(n, σ') := update_input σ in *) *)
-(*   (*     Some ((Val (LitV n)), σ', K, (1, 1)) *) *)
-(*   (* | Output (Val (LitV n)) => *) *)
-(*   (*     (* let := update_output n σ in *) *) *)
-(*   (*     Some ((Val (LitV 0)), σ', K, (1, 1)) *) *)
-(*   | (NatOp op (Val v1) (Val v2)) => *)
-(*       let res := nat_op_interp op v1 v2 in *)
-(*       option_rect (fun _ => option _) (fun v3 => Some ((Val v3), K, (0, 0))) None res *)
-(*   | (If (Val (LitV n)) e1 e2) => *)
-(*       if (decide (0 < n)) *)
-(*       then Some (e1, K, (0, 0)) *)
-(*       else *)
-(*         if (decide (n = 0)) *)
-(*         then Some (e2, K, (0, 0)) *)
-(*         else None *)
-(*   (* | (Shift e) => *) *)
-(*   (*     let (Ki, Ko) := shift_context K in *) *)
-(*   (*     let f := cont_to_rec Ki in *) *)
-(*   (*     Some ((subst (Inc := inc) e (Val f)), Ko, (1, 1)) *) *)
-(*   | (Reset (Val v)) => Some (Val v, K, (1, 1)) *)
-(*   (* | (Reset (fill E (Shift e))) => None *) *)
-(*   | _ => None *)
-(*   end. *)
-(* (* CHECK *) *)
-
-(* Example test21 : val ∅ := (rec (if ($ 0) then # 1 else #0))%syn. *)
-
-
-(* Example testc : option (expr (inc ∅) * cont (inc ∅) * (nat * nat)) := *)
-(*   (compute_head_step (App (Val test1) (Val $ LitV 5)) []). *)
-(* Eval compute in testc. *)
-
-
-(* Lemma head_step_reflect {S : Set} (e : expr S) (K Ko : cont S) *)
-(*   : option_reflect (fun '(e', K', nm) => head_step e K e' K' Ko nm) *)
-(*       True *)
-(*       (compute_head_step e  K). *)
-(* Proof. *)
-(*   destruct e; try (by constructor). *)
-(*   - destruct e1; try (by constructor). *)
-(*     destruct v; try (by constructor). *)
-(*     destruct e2; try (by constructor). *)
-(*     constructor. *)
-(*     constructor. *)
-(*   - destruct e1; try (by constructor). *)
-(*     destruct e2; try (by constructor). *)
-(*     destruct (nat_op_interp op v v0) eqn:Heqn. *)
-(*     + simpl; rewrite Heqn. *)
-(*       simpl. *)
-(*       constructor. *)
-(*       by constructor. *)
-(*     + simpl; rewrite Heqn. *)
-(*       simpl. *)
-(*       constructor. *)
-(*       constructor. *)
-(*   - destruct e1; try (by constructor). *)
-(*     destruct v; try (by constructor). *)
-(*     simpl. *)
-(*     case_match; simpl. *)
-(*     + constructor. *)
-(*       constructor. *)
-(*       assumption. *)
-(*     + case_match; simpl. *)
-(*       * constructor. *)
-(*         constructor. *)
-(*         assumption. *)
-(*       * constructor. *)
-(*         constructor. *)
-(*   (* - simpl. *) *)
-(*   (*   destruct (update_input σ) eqn:Heqn. *) *)
-(*   (*   by do 2 constructor. *) *)
-(*   (* - simpl. *) *)
-(*   (*   destruct e; try (by constructor). *) *)
-(*   (*   destruct v; try (by constructor). *) *)
-(*   (*   destruct (update_output n σ) eqn:Heqn. *) *)
-(*   (*   by do 2 constructor. *) *)
-(*   (* - simpl. *) *)
-(*   (*   destruct (shift_context K) as [Ki Ko] eqn:HK. *) *)
-(*   (*   constructor. apply ShiftS with Ki =>//=. *) *)
-(*   -  simpl. *)
-(*      destruct e; try (by constructor). *)
-(*      do 2 constructor. *)
-(* Qed. *)
