theories/examples/delim_lang/adeq.v
@@ -1,0 +1,750 @@
+From gitrees Require Import gitree lang_generic hom.
+From gitrees.effects Require Import delim.
+From gitrees.examples.delim_lang Require Import lang interp.
+From iris.algebra Require Import list.
+From iris.proofmode Require Import classes tactics.
+From iris.base_logic Require Import algebra.
+
+Require Import Binding.Lib Binding.Set Binding.Env.
+
+Open Scope syn.
+
+Inductive ty :=
+| Tnat : ty
+| Tarr : ty -> ty -> ty -> ty -> ty
+| Tcont : ty → ty → ty.
+
+Declare Scope types.
+
+Notation "τ '∕' α '→' σ '∕' β" := (Tarr τ α σ β) (at level 60) : types.
+Notation "'Cont' τ σ" := (Tcont τ σ) (at level 60) : types.
+
+Reserved Notation "Γ ';' α '⊢ₑ' e ':' τ ';' β"
+  (at level 90, e at next level, τ at level 20, no associativity).
+
+Reserved Notation "Γ ';' α '⊢ᵥ' e ':' τ ';' β"
+  (at level 90, e at next level, τ at level 20, no associativity).
+
+Reserved Notation "Γ ';' α '⊢ᵪ' e ':' τ ';' β"
+  (at level 90, e at next level, τ at level 20, no associativity).
+
+(* TODO: pure stuff has ∀ σ deeper inside *)
+Inductive typed_expr {S : Set} (Γ : S -> ty) : ty -> expr S -> ty -> ty -> Prop :=
+| typed_Val v α τ β :
+  (Γ; α ⊢ᵥ v : τ; β) →
+  (Γ; α ⊢ₑ v : τ; β)
+| typed_Var x τ α :
+  (Γ x = τ) →
+  (Γ; α ⊢ₑ (Var x) : τ; α)
+| typed_App e₁ e₂ γ α β δ σ τ :
+  (Γ; γ ⊢ₑ e₁ : (Tarr σ α τ β); δ) →
+  (Γ; β ⊢ₑ e₂ : σ; γ) →
+  (Γ; α ⊢ₑ (App e₁ e₂) : τ; δ)
+| typed_AppCont e₁ e₂ α β δ σ τ :
+  (Γ; δ ⊢ₑ e₁ : (Tcont τ α); β) →
+  (Γ; σ ⊢ₑ e₂ : τ; δ) →
+  (Γ; σ ⊢ₑ (AppCont e₁ e₂) : α; β)
+| typed_NatOp o e₁ e₂ α β :
+  (Γ; α ⊢ₑ e₁ : Tnat; β) →
+  (Γ; α ⊢ₑ e₂ : Tnat; β) →
+  (Γ; α ⊢ₑ NatOp o e₁ e₂ : Tnat; β)
+| typed_If e e₁ e₂ α β σ τ :
+  (Γ; σ ⊢ₑ e : Tnat; β) →
+  (Γ; α ⊢ₑ e₁ : τ; σ) →
+  (Γ; α ⊢ₑ e₂ : τ; σ) →
+  (Γ; α ⊢ₑ (if e then e₁ else e₂) : τ; β)
+| typed_Shift (e : @expr (inc S)) τ α σ β :
+  (Γ ▹ (Tcont τ α); σ ⊢ₑ e : σ; β) →
+  (Γ; α ⊢ₑ Shift e : τ; β)
+| typed_Reset e α σ τ :
+  (Γ; σ ⊢ₑ e : σ; τ) →
+  (Γ; α ⊢ₑ reset e : τ; α)
+where "Γ ';' α '⊢ₑ' e ':' τ ';' β" := (typed_expr Γ α e τ β) : types
+with typed_val {S : Set} (Γ : S -> ty) : ty -> val S -> ty -> ty -> Prop :=
+| typed_LitV n α :
+  (Γ; α ⊢ᵥ #n : Tnat; α)
+| typed_RecV (e : expr (inc (inc S))) (δ σ τ α β : ty) :
+  ((Γ ▹ (Tarr σ α τ β) ▹ σ); α ⊢ₑ e : τ; β) ->
+  (Γ; δ ⊢ᵥ (RecV e) : (Tarr σ α τ β); δ)
+| typed_ContV (k : cont S) τ α β :
+  (Γ; α ⊢ᵪ k : τ; β) →
+  (Γ; α ⊢ᵥ (ContV k) : τ; β)
+where "Γ ';' α '⊢ᵥ' e ':' τ ';' β" := (typed_val Γ α e τ β) : types
+with typed_cont {S : Set} (Γ : S -> ty) : ty -> cont S -> ty -> ty -> Prop :=
+| typed_END τ δ :
+  (Γ; δ ⊢ᵪ END : (Tcont τ τ); δ)
+| typed_IfK e₁ e₂ α β δ A k τ :
+  (Γ; α ⊢ₑ e₁ : τ; β) ->
+  (Γ; α ⊢ₑ e₂ : τ; β) ->
+  (Γ; β ⊢ᵪ k : Tcont τ A; δ) ->
+  (Γ; α ⊢ᵪ IfK e₁ e₂ k : Tcont Tnat A; δ)
+(* | typed_AppLK v k α β σ δ τ' τ : *)
+(*   (Γ; α ⊢ᵥ v : τ'; β) -> *)
+(*   (Γ; β ⊢ᵪ k : Tcont σ τ; δ) -> *)
+(*   (Γ; α ⊢ᵪ AppLK v k : Tcont (Tarr τ' α σ δ) τ; δ) *)
+(* | typed_AppRK e k τ : *)
+(*   (Γ; τ ⊢ᵪ AppRK e k : τ; τ) *)
+(* | typed_AppContLK v k τ : *)
+(*   (Γ; τ ⊢ᵪ AppContLK v k : τ; τ) *)
+(* | typed_AppContRK e k τ : *)
+(*   (Γ; τ ⊢ᵪ AppContRK e k : τ; τ) *)
+| typed_NatOpLK op v k α β δ τ :
+  (Γ; α ⊢ᵥ v : Tnat; β) ->
+  (Γ; β ⊢ᵪ k : Tcont Tnat τ; δ) ->
+  (Γ; α ⊢ᵪ NatOpLK op v k : Tcont Tnat τ; δ)
+| typed_NatOpRK op e k α β δ τ :
+  (Γ; α ⊢ₑ e : Tnat; β) ->
+  (Γ; β ⊢ᵪ k : Tcont Tnat τ; δ) ->
+  (Γ; α ⊢ᵪ NatOpRK op e k : Tcont Tnat τ; δ)
+where "Γ ';' α '⊢ᵪ' e ':' τ ';' β" := (typed_cont Γ α e τ β) : types
+.
+
+Open Scope stdpp_scope.
+
+Section logrel.
+  Context {sz : nat}.
+  Variable (rs : gReifiers CtxDep sz).
+  Context {R} `{!Cofe R}.
+  Context `{!SubOfe natO R}.
+  Context `{!subReifier reify_delim rs}.
+  Notation F := (gReifiers_ops rs).
+  Notation IT := (IT F R).
+  Notation ITV := (ITV F R).
+  Context `{!invGS Σ}.
+  Context `{!stateG rs R Σ}.
+  Notation iProp := (iProp Σ).
+  Notation restO := (gState_rest
+                       (@sR_idx _ _
+                          (sReifier_NotCtxDep_CtxDep reify_delim)) rs ♯ IT).
+
+  Canonical Structure exprO S := leibnizO (expr S).
+  Canonical Structure valO S := leibnizO (val S).
+  Canonical Structure contO S := leibnizO (cont S).
+
+  Notation "'WP' α {{ β , Φ } }" := (wp rs α notStuck ⊤ (λ β, Φ))
+                                      (at level 20, α, Φ at level 200,
+                                        format "'WP'  α  {{  β ,  Φ  } }")
+      : bi_scope.
+
+  Notation "'WP' α {{ Φ } }" := (wp rs α notStuck ⊤ Φ)
+                                  (at level 20, α, Φ at level 200,
+                                    format "'WP'  α  {{  Φ  } }") : bi_scope.
+
+  Definition logrel_nat' (βv : ITV) : iProp :=
+    (∃ (n : natO), βv ≡ RetV n)%I.
+  Local Instance logrel_nat_ne : NonExpansive logrel_nat'.
+  Proof. solve_proper. Qed.
+  Definition logrel_nat : ITV -n> iProp := λne x, logrel_nat' x.
+
+  (* --------- *)
+  (* Program Definition logrel_expr' *)
+  (*   (f : (ITV -n> iProp) -n> (ITV -n> iProp) -n> ITV -n> iProp) *)
+  (*   (τ α β : ITV -n> iProp) *)
+  (*   (βe : IT) : iProp := *)
+  (*   (∀ (σ : stateF ♯ IT) (κ : HOM), *)
+  (*      f τ α (FunV (Next κ)) *)
+  (*      -∗ has_substate ((laterO_map κ :: σ) : sReifier_state reify_delim ♯ IT) *)
+  (*      -∗ WP (𝒫 βe) {{ βv, β βv ∗ has_substate σ }})%I. *)
+  (* Local Instance logrel_expr_ne *)
+  (*   : (∀ n, Proper (dist n *)
+  (*                     ==> dist n *)
+  (*                     ==> dist n *)
+  (*                     ==> dist n *)
+  (*                     ==> dist n *)
+  (*                     ==> dist n) *)
+  (*             logrel_expr'). *)
+  (* Proof. solve_proper. Qed. *)
+  (* Program Definition logrel_expr *)
+  (*   : ((ITV -n> iProp) -n> (ITV -n> iProp) -n> ITV -n> iProp) *)
+  (*     -n> (ITV -n> iProp) -n> (ITV -n> iProp) -n> (ITV -n> iProp) *)
+  (*                                                 -n> IT -n> iProp := *)
+  (*   λne x y z w v, logrel_expr' x y z w v. *)
+  (* Solve All Obligations with solve_proper. *)
+
+  (* Program Definition logrel_cont_pre *)
+  (*   : ((ITV -n> iProp) -n> (ITV -n> iProp) -n> ITV -n> iProp) *)
+  (*     -n> ((ITV -n> iProp) -n> (ITV -n> iProp) -n> ITV -n> iProp) := *)
+  (*   λne μ τ α βv, *)
+  (*   (∃ (f : HOM), (IT_of_V βv) ≡ (Fun (Next f)) *)
+  (*                 ∧ □ ∀ αv, τ αv → ∀ (β : ITV -n> iProp), *)
+  (*      ▷ (logrel_expr μ α β β (`f (IT_of_V αv))))%I. *)
+  (* Solve All Obligations with solve_proper. *)
+
+  (* Local Instance logrel_cont_pre_contr : Contractive logrel_cont_pre. *)
+  (* Proof. solve_contractive. Qed. *)
+
+  (* Definition logrel_cont : (ITV -n> iProp) -n> (ITV -n> iProp) -n> ITV -n> iProp *)
+  (*   := fixpoint logrel_cont_pre. *)
+  (* Lemma logrel_cont_unfold τ α βv : *)
+  (*   logrel_cont τ α βv *)
+  (*     ≡ ((∃ (f : HOM), (IT_of_V βv) ≡ (Fun (Next (`f))) *)
+  (*                      ∧ □ ∀ αv, τ αv → ∀ (β : ITV -n> iProp), *)
+  (*           ▷ (logrel_expr logrel_cont α β β (`f (IT_of_V αv))))%I). *)
+  (* Proof. apply (fixpoint_unfold logrel_cont_pre _). Qed. *)
+
+  (* Program Definition logrel_arr' (τ α σ β : ITV -n> iProp) (βf : ITV) : iProp := *)
+  (*   (∃ f, IT_of_V βf ≡ Fun f *)
+  (*         ∧ □ ∀ (βv : ITV), *)
+  (*      τ βv -∗ logrel_expr logrel_cont σ α β (APP' (Fun f) (IT_of_V βv)))%I. *)
+  (* Local Instance logrel_arr_ne *)
+  (*   : (∀ n, Proper (dist n *)
+  (*                     ==> dist n *)
+  (*                     ==> dist n *)
+  (*                     ==> dist n *)
+  (*                     ==> dist n *)
+  (*                     ==> dist n) *)
+  (*             logrel_arr'). *)
+  (* Proof. solve_proper. Qed. *)
+  (* Program Definition logrel_arr *)
+  (*   : (ITV -n> iProp) *)
+  (*     -n> (ITV -n> iProp) *)
+  (*         -n> (ITV -n> iProp) *)
+  (*             -n> (ITV -n> iProp) -n> ITV -n> iProp := *)
+  (*   λne x y z w v, logrel_arr' x y z w v. *)
+  (* Solve All Obligations with solve_proper. *)
+
+  (* Fixpoint interp_ty (τ : ty) : ITV -n> iProp := *)
+  (*   match τ with *)
+  (*   | Tnat => logrel_nat *)
+  (*   | Tcont α β => logrel_cont (interp_ty α) (interp_ty β) *)
+  (*   | Tarr τ α σ β => logrel_arr (interp_ty τ) (interp_ty α) *)
+  (*                      (interp_ty σ) (interp_ty β) *)
+  (*   end. *)
+
+  (* Definition logrel (τ α β : ty) : IT -n> iProp *)
+  (*   := logrel_expr logrel_cont (interp_ty τ) (interp_ty α) (interp_ty β). *)
+
+  (* Local Instance interp_ty_persistent (τ : ty) α : *)
+  (*   Persistent (interp_ty τ α). *)
+  (* Proof. *)
+  (*   revert α. induction τ=> α; simpl. *)
+  (*   - unfold logrel_nat. apply _. *)
+  (*   - unfold logrel_arr. apply _. *)
+  (*   - unfold logrel_cont. *)
+  (*     rewrite logrel_cont_unfold. *)
+  (*     apply _. *)
+  (* Qed. *)
+  (* ---- *)
+
+  (* -------------------------------------- *)
+
+  Program Definition has_cont_stack : stateF ♯ IT -> iProp := λ σ,
+      (has_substate (σ : sReifier_state reify_delim ♯ IT)
+       ∗ ([∗ list] (x : laterO IT -n> laterO IT) ∈ σ,
+           ∃ (κ : HOM), x ≡ (laterO_map κ)))%I.
+
+  Lemma wp_shift (σ : stateF ♯ IT) (f : (laterO IT -n> laterO IT) -n> laterO IT)
+    (k : IT -n> IT) β {Hk : IT_hom k} Φ :
+    laterO_map 𝒫 (f (laterO_map k)) ≡ Next β →
+    has_cont_stack σ -∗
+    ▷ (£ 1 -∗ has_cont_stack σ -∗ WP β {{ Φ }}) -∗
+    WP (k (SHIFT f)) {{ Φ }}.
+  Proof.
+    iIntros (Hp) "(Hs & G) Ha".
+    iApply (wp_shift with "[Hs]"); [done | done |].
+    iNext.
+    iIntros "HCr Hs".
+    iApply ("Ha" with "HCr").
+    iFrame.
+  Qed.
+
+  Lemma wp_reset (σ : stateF ♯ IT) (e : IT) (k : IT -n> IT) {Hk : IT_hom k}
+    Φ :
+    has_cont_stack σ -∗
+    ▷ (£ 1 -∗ has_cont_stack ((laterO_map k) :: σ) -∗
+       WP 𝒫 e {{ Φ }}) -∗
+    WP k $ (RESET (Next e)) {{ Φ }}.
+  Proof.
+    iIntros "(Hs & G) Ha".
+    iApply (wp_reset with "[Hs]"); [done |].
+    iNext.
+    iIntros "HCr Hs".
+    iApply ("Ha" with "HCr").
+    iFrame.
+    unshelve eset (F := exist _ k _ : HOM); first done.
+    iExists F.
+    now subst F.
+  Qed.
+
+  Lemma wp_pop_end (v : IT)
+    {HV : AsVal v}
+    Φ :
+    has_cont_stack [] -∗
+    ▷ (£ 1 -∗ has_cont_stack [] -∗ WP v {{ Φ }}) -∗
+    WP 𝒫 v {{ Φ }}.
+  Proof.
+    iIntros "(Hs & G) Ha".
+    iApply (wp_pop_end with "Hs").
+    iNext.
+    iIntros "HCr Hs".
+    iApply ("Ha" with "HCr").
+    now iFrame.
+  Qed.
+
+  Lemma wp_pop_cons (σ : stateF ♯ IT) (v : IT) (k : IT -n> IT)
+    {HV : AsVal v}
+    Φ :
+    has_cont_stack ((laterO_map k) :: σ) -∗
+    ▷ (£ 1 -∗ has_cont_stack σ -∗ WP k $ v {{ Φ }}) -∗
+    WP 𝒫 v {{ Φ }}.
+  Proof.
+    iIntros "(Hs & (_ & G)) Ha".
+    iApply (wp_pop_cons with "Hs").
+    iNext.
+    iIntros "HCr Hs".
+    iApply ("Ha" with "HCr").
+    iFrame.
+  Qed.
+
+  Lemma wp_app_cont (σ : stateF ♯ IT) (e : laterO IT) (k' : laterO (IT -n> IT))
+    (k : IT -n> IT) β {Hk : IT_hom k}
+    Φ :
+    laterO_ap k' e ≡ Next β →
+    has_cont_stack σ -∗
+    ▷ (£ 1 -∗ has_cont_stack ((laterO_map k) :: σ) -∗
+       WP β {{ Φ }}) -∗
+    WP k (APP_CONT e k') {{ Φ }}.
+  Proof.
+    iIntros (Hb) "(Hs & G) Ha".
+    iApply (wp_app_cont with "Hs");
+      first done.
+    iNext.
+    iIntros "HCr Hs".
+    iApply ("Ha" with "HCr").
+    iFrame.
+    unshelve eset (F := exist _ k _ : HOM); first done.
+    iExists F.
+    now subst F.
+  Qed.
+
+  Definition obs_ref' (P : ITV -n> iProp) (t : IT) : iProp :=
+    (∀ (σ : stateF ♯ IT),
+       has_cont_stack σ
+       -∗ WP t {{ βv, ∃ σ',
+                        P βv ∗ has_cont_stack σ' }})%I.
+  Local Instance obs_ref_ne : NonExpansive2 obs_ref'.
+  Proof. solve_proper. Qed.
+  Program Definition obs_ref : (ITV -n> iProp) -n> IT -n> iProp :=
+    λne x y, obs_ref' x y.
+  Solve All Obligations with solve_proper.
+
+  Program Definition logrel_cont'
+    (Pτ Pα : ITV -n> iProp) (k : ITV)
+    : iProp :=
+    (∃ (f : HOM),
+       (IT_of_V k) ≡ (Fun (Next f))
+       ∧ □ ∀ αv, Pτ αv -∗ obs_ref Pα ((`f) (IT_of_V αv)))%I.
+  Local Instance logrel_cont_ne : NonExpansive3 logrel_cont'.
+  Proof. solve_proper. Qed.
+  Program Definition logrel_cont
+    : (ITV -n> iProp) -n> (ITV -n> iProp) -n> ITV -n> iProp :=
+    λne x y z, logrel_cont' x y z.
+  Solve All Obligations with solve_proper.
+
+  Program Definition logrel_expr' (Pτ Pα Pβ : ITV -n> iProp)
+    (e : IT) : iProp :=
+    (∀ (σ : stateF ♯ IT) (κ : HOM),
+       logrel_cont Pτ Pα (FunV (Next κ))
+       -∗ has_cont_stack ((laterO_map κ :: σ) : sReifier_state reify_delim ♯ IT)
+       -∗ WP (𝒫 e) {{ βv, ∃ σ', Pβ βv ∗ has_cont_stack σ' }})%I.
+  Local Instance logrel_expr_ne : NonExpansive4 logrel_expr'.
+  Proof. solve_proper. Qed.
+  Program Definition logrel_expr
+    : (ITV -n> iProp) -n> (ITV -n> iProp) -n> (ITV -n> iProp) -n> IT -n> iProp :=
+    λne x y z w, logrel_expr' x y z w.
+  Solve All Obligations with solve_proper.
+
+  Program Definition logrel_arr' (Pτ Pα Pσ Pβ : ITV -n> iProp) (f : ITV) : iProp :=
+    (∃ f', IT_of_V f ≡ Fun f'
+          ∧ □ ∀ (βv : ITV),
+       Pτ βv -∗ logrel_expr Pσ Pα Pβ (APP' (Fun f') (IT_of_V βv)))%I.
+  Local Instance logrel_arr_ne
+    : (∀ n, Proper (dist n
+                      ==> dist n
+                      ==> dist n
+                      ==> dist n
+                      ==> dist n
+                      ==> dist n)
+              logrel_arr').
+  Proof. solve_proper. Qed.
+  Program Definition logrel_arr
+    : (ITV -n> iProp)
+      -n> (ITV -n> iProp)
+          -n> (ITV -n> iProp)
+              -n> (ITV -n> iProp) -n> ITV -n> iProp :=
+    λne x y z w v, logrel_arr' x y z w v.
+  Solve All Obligations with solve_proper.
+
+  Fixpoint interp_ty (τ : ty) : ITV -n> iProp :=
+    match τ with
+    | Tnat => logrel_nat
+    | Tcont α β => logrel_cont (interp_ty α) (interp_ty β)
+    | Tarr τ α σ β => logrel_arr (interp_ty τ) (interp_ty α)
+                       (interp_ty σ) (interp_ty β)
+    end.
+
+  Local Instance interp_ty_persistent (τ : ty) α :
+    Persistent (interp_ty τ α).
+  Proof.
+    revert α. induction τ=> α; simpl.
+    - unfold logrel_nat. apply _.
+    - unfold logrel_arr. apply _.
+    - unfold logrel_cont. apply _.
+  Qed.
+
+  Definition logrel (τ α β : ty) : IT -n> iProp
+    := logrel_expr (interp_ty τ) (interp_ty α) (interp_ty β).
+
+  Program Definition ssubst_valid {S : Set}
+    (Γ : S -> ty)
+    (ss : interp_scope S) : iProp :=
+    (∀ x α, □ logrel (Γ x) α α (ss x))%I.
+
+  (* TODO: continuation *)
+  Program Definition valid {S : Set}
+    (Γ : S -> ty)
+    (e : interp_scope S -n> IT)
+    (τ α β : ty) : iProp :=
+    (∀ γ, ssubst_valid Γ γ
+           -∗ logrel τ α β (e γ))%I.
+
+  Lemma compat_var {S : Set} (Γ : S -> ty) (x : S) :
+    ⊢ (∀ α, valid Γ (interp_var x) (Γ x) α α).
+  Proof.
+    iIntros (α γ) "Hss".
+    iApply "Hss".
+  Qed.
+
+  Lemma logrel_of_val τ α v :
+    interp_ty τ v -∗ logrel τ α α (IT_of_V v).
+  Proof.
+    iIntros "#H".
+    iIntros (σ κ) "#Hκ".
+    iIntros "Hs".
+    iApply (wp_pop_cons with "Hs").
+    iDestruct "Hκ" as "(%f & #HEQ & Hκ)".
+    iPoseProof (Fun_inj' with "HEQ") as "HEQ'".
+    iNext.
+    iIntros "HCr Hσ".
+    unshelve eset (F := (λne βv, interp_ty α βv)%I : ITV -n> iProp);
+      first solve_proper.
+    iSpecialize ("Hκ" $! v with "H").
+    iSpecialize ("Hκ" $! σ with "Hσ").
+    subst F.
+    iAssert ((`κ) (IT_of_V v) ≡ (`f) (IT_of_V v))%I as "HEQ''".
+    {
+      unshelve iApply (f_equivI (λne (f : IT -n> IT),
+                           f (IT_of_V v)) (`κ) (`f) with "HEQ'"); solve_proper.
+    }
+    iRewrite "HEQ''".
+    iExact "Hκ".
+  Qed.
+
+  Lemma compat_recV {S : Set} (Γ : S -> ty)
+    τ1 α τ2 β e :
+    ⊢ □ valid ((Γ ▹ (Tarr τ1 α τ2 β) ▹ τ1)) e τ2 α β
+      -∗ (∀ θ, valid Γ (interp_rec rs e) (Tarr τ1 α τ2 β) θ θ).
+  Proof.
+    iIntros "#H".
+    iIntros (θ γ) "#Henv".
+    set (f := (ir_unf rs e γ)).
+    iAssert (interp_rec rs e γ ≡ IT_of_V $ FunV (Next f))%I as "Hf".
+    { iPureIntro. apply interp_rec_unfold. }
+    iRewrite "Hf".
+    Opaque IT_of_V.
+    iApply logrel_of_val; term_simpl.
+    iExists _. iSplit.
+    { iPureIntro. apply into_val. }
+    iModIntro.
+    iLöb as "IH".
+    iIntros (v) "#Hw".
+    iIntros (σ κ) "#Hκ Hσ".
+    rewrite APP_APP'_ITV APP_Fun laterO_map_Next -Tick_eq.
+    pose (γ' := (extend_scope (extend_scope γ (interp_rec rs e γ)) (IT_of_V v))).
+    rewrite /logrel.
+    iSpecialize ("H" $! γ' with "[Hw]").
+    {
+      iIntros (x).
+      destruct x as [| [| x]]; iIntros (ξ); iModIntro.
+      * iApply logrel_of_val.
+        iApply "Hw".
+      * simpl.
+        iRewrite "Hf".
+        iIntros (σ' κ') "Hκ' Hσ'".
+        iApply (wp_pop_cons with "Hσ'").
+        iDestruct "Hκ'" as "(%g & #HEQ & Hκ')".
+        Transparent IT_of_V.
+        iDestruct (Fun_inj' with "HEQ") as "HEQ'".
+        iNext.
+        iIntros "HCr Hσ'".
+        iSpecialize ("Hκ'" $! (FunV (Next f))).
+        iSpecialize ("Hκ'" with "[]").
+        {
+          iExists (Next f).
+          iSplit; first done.
+          iModIntro.
+          iIntros (v') "Hv'".
+          by iApply "IH".
+        }
+        iSpecialize ("Hκ'" $! σ' with "Hσ'").
+        iAssert ((`κ') (IT_of_V (FunV (Next f)))
+                   ≡ (`g) (IT_of_V (FunV (Next f))))%I as "HEQ''".
+        {
+          unshelve iPoseProof
+            (f_equivI (λne (f' : IT -n> IT),
+                 f' (Fun (Next f))) (`κ') (`g) with "[HEQ']") as "GGG";
+            first solve_proper; first solve_proper; first done.
+          iApply "GGG".
+        }
+        simpl.
+        iRewrite "HEQ''".
+        iExact "Hκ'".
+      * iApply "Henv".
+    }
+    Opaque extend_scope.
+    simpl.
+    rewrite hom_tick.
+    iApply wp_tick.
+    iNext.
+    subst γ'.
+    iApply ("H" with "Hκ Hσ").
+  Qed.
+
+  Program Definition 𝒫_HOM : @HOM sz CtxDep R _ _ := exist _ 𝒫 _.
+  Next Obligation. apply _. Qed.
+
+  Lemma compat_reset {S : Set} (Γ : S -> ty) e σ τ :
+        ⊢ valid Γ e σ σ τ -∗ (∀ α, valid Γ (interp_reset rs e) τ α α).
+  Proof.
+    iIntros "H".
+    iIntros (α γ) "#Henv".
+    iIntros (σ' κ) "#Hκ Hσ'".
+    iApply (wp_reset with "Hσ'").
+    iNext.
+    iIntros "HCr Hσ'".
+    iSpecialize ("H" $! γ with "Henv").
+    iSpecialize ("H" $! (laterO_map (`κ) :: σ') 𝒫_HOM with "[] Hσ'").
+    {
+      iExists 𝒫_HOM.
+      iSplit; first done.
+      iModIntro.
+      iIntros (v) "#Hv".
+      iIntros (σ'') "Hσ''".
+      destruct σ'' as [| κ' σ''].
+      - simpl.
+        iApply (wp_pop_end with "Hσ''").
+        iNext.
+        iIntros "HC Hs".
+        iApply wp_val.
+        iModIntro.
+        iExists [].
+        iFrame "Hs Hv".
+      - simpl.
+        simpl in κ'.
+        iDestruct "Hσ''" as "(H1 & #H2)".
+        rewrite big_opL_cons.
+        iDestruct "H2" as "((%κκ & Hκκ) & H2)".
+        iRewrite "Hκκ" in "H1".
+        iApply (delim.wp_pop_cons with "H1").
+        iNext.
+        iIntros "HC Hs".
+        iDestruct "Hκ" as "(%g & #HEQ & #Hκ)".
+        iSpecialize ("Hκ" $! v).
+        (* pop cons different rule with extra tick *)
+        admit.
+    }
+    (* push continuation forward *)
+    iApply (wp_wand with "H").
+    iIntros (v) "(%s & #G1 & G2)".
+    iModIntro.
+    iExists s.
+    iFrame.
+    admit.
+  Admitted.
+
+  Lemma compat_shift {S : Set} (Γ : S -> ty) e σ α τ β :
+    ⊢ valid (Γ ▹ (Tcont τ α)) e σ σ β -∗ valid Γ (interp_shift _ e) τ α β.
+  Proof.
+    iIntros "H".
+    iIntros (γ) "#Henv".
+    iIntros (σ' κ) "#Hκ Hσ'".
+    iApply (wp_shift with "Hσ'").
+    { apply (laterO_map_Next 𝒫). }
+    {
+      iNext.
+      iIntros "HCr Hσ'".
+      set (F := (FunV (Next (λne x : IT, Tau (laterO_map 𝒫 (Next x))))) : ITV).
+      iSpecialize ("H" $! (extend_scope γ (IT_of_V F)) with "[Hκ]").
+      - iIntros (x τ').
+        iDestruct "Hκ" as "(%g & #HEQ & #Hκ)".
+        iIntros (σ'' κ').
+        iModIntro.
+        iIntros "Hκ' Hσ''".
+        destruct x as [| x].
+        + Transparent extend_scope.
+          iApply (wp_pop_cons with "Hσ''").
+          iDestruct (Fun_inj' with "HEQ") as "HEQ''".
+          iDestruct "Hκ'" as "(%h & #HEQ' & #Hκ')".
+          iDestruct (Fun_inj' with "HEQ'") as "HEQ'''".
+          iSpecialize ("Hκ'" $! F).
+          iNext.
+          iIntros "HCr Hs".
+          iApply (wp_wand with "[Hκ' Hs]").
+          {
+            iAssert ((`κ') (extend_scope γ (IT_of_V F) VZ)
+                       ≡ (`h) (extend_scope γ (IT_of_V F) VZ))%I as "HEQ''''".
+            {
+              unshelve iPoseProof (f_equivI (λne (f' : IT -n> IT), f' (extend_scope γ (IT_of_V F) VZ)) (`κ') (`h) with "[HEQ']") as "GGG";
+                first solve_proper; first solve_proper;
+                first done.
+              iApply "GGG".
+            }
+            iRewrite "HEQ''''".
+            iApply "Hκ'"; last iApply "Hs".
+            simpl.
+            unfold logrel_cont'.
+            subst F.
+            unshelve eset (F' := exist _ (λne x : IT, Tau (laterO_map 𝒫 (Next x))) _ : HOM).
+            {
+              simpl.
+              econstructor.
+              - intros.
+                rewrite ->2 later_map_Next.
+                rewrite hom_tick.
+                rewrite <- Tick_eq.
+                rewrite <- Tick_eq.
+                reflexivity.
+              - intros.
+                rewrite -> later_map_Next.
+                rewrite hom_vis.
+                rewrite <- Tick_eq.
+                admit.
+              - intros.
+                rewrite -> later_map_Next.
+                rewrite hom_err.
+                admit.
+            }
+            iExists F'.
+            iSplit; first done.
+            iModIntro.
+            iIntros (v) "HHH".
+            subst F'.
+            simpl.
+            rewrite later_map_Next.
+            iIntros (s) "Hs".
+            rewrite <- Tick_eq.
+            iApply wp_tick.
+            iNext.
+            destruct s as [| x s].
+            - iApply (wp_pop_end with "Hs").
+              iNext.
+              iIntros "HCr Hs".
+              iApply wp_val.
+              iModIntro.
+              iExists [].
+              iFrame "Hs".
+              admit.
+            - admit.
+          }
+          iIntros (v) "HHH".
+          iModIntro.
+          iApply "HHH".
+        + iApply ("Henv" with "[Hκ'] Hσ''").
+          iApply "Hκ'".
+      - subst F.
+        Opaque extend_scope.
+        simpl.
+        unfold logrel_expr'.
+        simpl.
+        iSpecialize ("H" $! σ' κ).
+
+        admit.
+    }
+  Admitted.
+
+  Lemma compat_appcont {S : Set} (Γ : S -> ty) e1 e2 τ α δ β σ :
+    valid Γ e1 (Tcont τ α) δ β
+    -∗ valid Γ e2 τ σ δ
+    -∗ valid Γ (interp_app_cont _ e1 e2) α σ β.
+  Proof.
+    iIntros "H G".
+    iIntros (γ) "#Henv".
+    iIntros (σ' κ) "#Hκ Hσ'".
+    iSpecialize ("H" $! γ with "Henv").
+    iSpecialize ("G" $! γ with "Henv").
+    iSpecialize ("H" $! σ').
+    iSpecialize ("G" $! σ').
+    (* (* bind + pop *) *)
+    admit.
+  Admitted.
+
+End logrel.
+
+Local Definition rs : gReifiers CtxDep 1 := gReifiers_cons reify_delim gReifiers_nil.
+
+Variable Hdisj : ∀ (Σ : gFunctors) (P Q : iProp Σ), disjunction_property P Q.
+
+Lemma logpred_adequacy cr Σ R `{!Cofe R, SubOfe natO R}
+  `{!invGpreS Σ} `{!statePreG rs R Σ} τ β'
+  (α : interp_scope ∅ -n> IT (gReifiers_ops rs) R)
+  (β : IT (gReifiers_ops rs) R) st st' k :
+  (∀ `{H1 : !invGS Σ} `{H2: !stateG rs R Σ},
+      (£ cr ⊢ valid rs □ α τ τ β')%I) →
+  ssteps (gReifiers_sReifier rs) (𝒫 (α ı_scope)) st β st' k →
+  (∃ β1 st1, sstep (gReifiers_sReifier rs) β st' β1 st1)
+   ∨ (∃ βv, IT_of_V βv ≡ β).
+Proof.
+  intros Hlog Hst.
+  destruct (IT_to_V β) as [βv|] eqn:Hb.
+  { right. exists βv. apply IT_of_to_V'. rewrite Hb; eauto. }
+  left.
+  cut ((∃ β1 st1, sstep (gReifiers_sReifier rs) β st' β1 st1)
+      ∨ (∃ e, β ≡ Err e ∧ notStuck e)).
+  { intros [?|He]; first done.
+    destruct He as [? [? []]]. }
+  eapply (wp_safety cr); eauto.
+  { apply Hdisj. }
+  { by rewrite Hb. }
+  intros H1 H2.
+  exists (λ _, True)%I. split. (* (interp_ty _ τ)%I *)
+  { apply _. }
+  iIntros "[Hcr  Hst]".
+  iPoseProof (Hlog with "Hcr") as "Hlog".
+  destruct st as [σ []].
+  iAssert (has_substate σ) with "[Hst]" as "Hs".
+  { unfold has_substate, has_full_state.
+    assert (of_state rs (IT (gReifiers_ops rs) _) (σ,()) ≡
+            of_idx rs (IT (gReifiers_ops rs) _) sR_idx (sR_state σ)) as ->; last done.
+    intro j. unfold sR_idx. simpl.
+    unfold of_state, of_idx.
+    destruct decide as [Heq|]; last first.
+    { inv_fin j; first done.
+      intros i. inversion i. }
+    inv_fin j; last done.
+    intros Heq.
+    rewrite (eq_pi _ _ Heq eq_refl)//.
+  }
+  iSpecialize ("Hlog" $! ı_scope with "[]").
+  { iIntros ([]). }
+  iSpecialize ("Hlog" $! σ HOM_id with "[]").
+  {
+    iExists HOM_id.
+    iSplit; first done.
+    iModIntro.
+    iIntros (αv) "HHH".
+    iIntros (βv) "Hκ".
+    simpl.
+    iApply wp_val.
+    iModIntro.
+    iExists βv.
+    iFrame.
+  }
+  iSpecialize ("Hlog" with "[Hs]").
+  {
+    admit.
+  }
+  iApply (wp_wand with "Hlog").
+  iIntros (βv). simpl.
+  iIntros "_".
+  done.
+Admitted.
