theories/hom.v
@@ -1,0 +1,50 @@
+From gitrees Require Import gitree lang_generic.
+Require Import Binding.Lib Binding.Set Binding.Env.
+
+Open Scope stdpp_scope.
+
+Section hom.
+  Context {sz : nat}.
+  Context {a : is_ctx_dep}.
+  Context {A : ofe}.
+  Context {CA : Cofe A}.
+  Context {rs : gReifiers a sz}.
+  Notation F := (gReifiers_ops rs).
+  Notation IT := (IT F A).
+  Notation ITV := (ITV F A).
+
+  Definition HOM : ofe := @sigO (IT -n> IT) IT_hom.
+
+  Global Instance HOM_hom (κ : HOM) : IT_hom (`κ).
+  Proof.
+    apply (proj2_sig κ).
+  Qed.
+
+  Program Definition HOM_id : HOM := exist _ idfun _.
+  Next Obligation.
+    apply _.
+  Qed.
+
+  Lemma HOM_ccompose (f g : HOM) :
+    ∀ α, `f (`g α) = (`f ◎ `g) α.
+  Proof.
+    intro; reflexivity.
+  Qed.
+
+  Program Definition HOM_compose (f g : HOM) : HOM := exist _ (`f ◎ `g) _.
+  Next Obligation.
+    intros f g; simpl.
+    apply _.
+  Qed.
+
+  Lemma HOM_compose_ccompose (f g h : HOM) :
+    h = HOM_compose f g ->
+    `f ◎ `g = `h.
+  Proof. intros ->. done. Qed.
+
+  Program Definition IFSCtx_HOM `{!SubOfe natO A} α β : HOM := exist _ (λne x, IFSCtx α β x) _.
+  Next Obligation.
+    intros; simpl.
+    apply _.
+  Qed.
+End hom.
